backend/CSEdomain.v
@@ -32,7 +32,7 @@ Definition valnum := positive.
 
 Inductive rhs : Type :=
   | Op: operation -> list valnum -> rhs
-  | Load: trapping_mode -> memory_chunk -> addressing -> list valnum -> rhs.
+  | Load: memory_chunk -> addressing -> list valnum -> rhs.
 
 Inductive equation : Type :=
   | Eq (v: valnum) (strict: bool) (r: rhs).
@@ -74,7 +74,7 @@ Definition empty_numbering :=
 Definition valnums_rhs (r: rhs): list valnum :=
   match r with
   | Op op vl => vl
-  | Load trap chunk addr vl => vl
+  | Load chunk addr vl => vl
   end.
 
 Definition wf_rhs (next: valnum) (r: rhs) : Prop :=
@@ -106,11 +106,11 @@ Inductive rhs_eval_to (valu: valuation) (ge: genv) (sp: val) (m: mem):
   | op_eval_to: forall op vl v,
       eval_operation ge sp op (map valu vl) m = Some v ->
       rhs_eval_to valu ge sp m (Op op vl) v
-  | load_eval_to: forall trap chunk addr vl a v,
+  | load_eval_to: forall chunk addr vl a v,
       eval_addressing ge sp addr (map valu vl) = Some a ->
       Mem.loadv chunk m a = Some v ->
-      rhs_eval_to valu ge sp m (Load trap chunk addr vl) v
-  | load_notrap1_eval_to: forall chunk addr vl,
+      rhs_eval_to valu ge sp m (Load chunk addr vl) v
+(*  | load_notrap1_eval_to: forall chunk addr vl,
       eval_addressing ge sp addr (map valu vl) = None ->
       rhs_eval_to valu ge sp m (Load NOTRAP chunk addr vl)
                   (default_notrap_load_value chunk)
@@ -118,7 +118,7 @@ Inductive rhs_eval_to (valu: valuation) (ge: genv) (sp: val) (m: mem):
       eval_addressing ge sp addr (map valu vl) = Some a ->
       Mem.loadv chunk m a = None ->
       rhs_eval_to valu ge sp m (Load NOTRAP chunk addr vl)
-                  (default_notrap_load_value chunk).
+                  (default_notrap_load_value chunk) *).
 
 Inductive equation_holds (valu: valuation) (ge: genv) (sp: val) (m: mem):
                                                       equation -> Prop :=
